Test/pruning/basic.bpl
@@ -1,4 +1,4 @@
-// RUN: %parallel-boogie "%s" > "%t"
+// RUN: %parallel-boogie /prune:2 "%s" > "%t"
 // RUN: %diff "%s.expect" "%t"
 
 type Ty;
@@ -11,9 +11,13 @@ const unique TagBool : TyTag uses {
     axiom Tag(TBool) == TagBool;
 }
 
-type Box;
-function $Box<T>(T): Box;
+function Magic<T>(x: T): T uses {
+    axiom (forall<T> x: T :: Magic(x) == 3);
+}
 
-function {:identity} Lit<T>(x: T): T { x } uses {
-    axiom (forall<T> x: T :: { $Box(Lit(x)) } $Box(Lit(x)) == Lit($Box(x)) );
+procedure test() 
+  ensures Magic(4) == 3;
+  ensures TagBool == Tag(TBool);
+{
+  
 }
